<<<
 List of properties of binomial coefficients in binomial expansion of (1 + x) raised to n
---


- Sum of binomial coefficients as \( 2^{n} \) 
- Equality of sum of coefficient of odd and even terms



>>> 
<<<
 Proof for sum of binomial coefficients of (1 +x) raised to n 
---

- $$ (1+x)^{n}= C(n,0) + C(n,1)x + C(n,2)x^{2} + . . . + C(n,n)x^{n} $$ 
- $$ \text{ x = 1 } $$
- $$ 2^{n} = C(n,0) + C(n,1) + C(n,2) + . . + C(n,n) $$ 


>>> 
<<<
 Expression for sum of coefficient of odd terms in binomial expansion of (1 +x) raised to n
---

$$ 2^{n-1} $$ 


>>> 
<<<
 Expression for sum of coefficient of even terms in binomial expansion of (1 +x) raised to n
---

$$ 2^{n-1} $$ 


>>> 
<<<
 Proof for expression of sum of coefficient of odd terms and sum of coefficient of even terms and their equality in binomial expansion of (1 +x) raised to n
---

- $$ (1 +x)^{n} = C_{0} + C_{1}x + C_{2}x^{2} + C_{3}x^{3} + .. .. .. + C_{n}x^{n}  $$ 
- $$ \text{x = -1} $$
- $$ (1-1)^{n} = C_{0} - C_{1} + C_{2} - C_{3} + C_{4} - .. .. .. .. $$ 
- $$ C_{0} + C_{2} + C_{4} + .. .. .. = C_{1} + C_{3} + C_{5} ..  $$
- $$ C_{0} + C_{1} + C_{2} + .. = 2^{n - 1} $$
- $$ C_{0} + C_{2} + C_{4} + .. .. .. = C_{1} + C_{3} + C_{5} .. = \frac{2^{n}}{2} = 2^{n -1} $$



>>> 
