Sum of first n natural numbers  : 
[latex]
\[
S_{n} =  1 + 2 + 3 + .. .. ..  + n \\
= \frac{n}{2}[2.1 +(n-1).1] \\
= \frac{n(n+1)}{2} \\
S_{n} = \frac{n(n+1)}{2}
\]
[/latex]

Sum of first n even natural numbers  : 
[latex]
\[
S_{n} =  2 + 4 + 6 + .. .. .. + n \\
S_{n} = 2( 1 + 2 + 3 + .. .. .. + n ) \\
S_{n} = 2n(n+1)\frac{1}{2} \\
S_{n} = n(n + 1)
\]
[/latex]

Sum of first n odd natural numbers  : 
[latex]
\[
S_{n} = 1 + 3 + 5 + .. .. .. + n \\
S_{n} = \frac{n}{2}[2.1 + (n-1).2] \\
S_{n} = n(1 + n -1) = n^{2}
\]
[/latex]

Identity for sum of square of first n natural numbers : 
[latex]
\[
r^{3} - ( r - 1 )^{3} \\
= r^{3} - (r^{3} -3r^{2} + 3r - 1) \\
= r^{3} - r^{3} + 3r^{2} -3r + 1\\
= 3r^{2} -3r + 1
\]
[/latex]

General term from identity sum of squares of first n natural numbers  : 
[latex]
\[
1^{3} - 0^{3} = 3.1^{2} - 3.1 + 1 \\
2^{3} - 1^{3} = 3.2^{2} - 3.2 + 1 \\
3^{3} - 2^{3} = 3.3^{2} - 3.3 + 1 \\
4^{3} - 3^{3} = 3.4^{2} - 3.4 + 1 \\
.. .. .. .. .. .. .. .. \\
n^{3} - (n-1)^{3} = 3n^{2} - 3n + 1
\]
[/latex]

Sum of squares of first n natural numbers : 
[latex]
\[
\text{Adding,} \\
n^{3} = 3(1^{2} + 2^{2} + 3^{2} + .. .. + n^{2}) -3(1 + 2 + 3 + .. + n) + n \\
n^{3} = 3S_{n} - 3 \times \frac{1}{2}n(n+1) + n \\
3S_{n} = n^{3} - n + \frac{3n(n+1)}{2} \\
= n(n^{2} -1) + \frac{3n(n+1)}{2} \\
= n(n+1)(n-1)+ \frac{3n(n+1)}{2} \\
= \frac{1}{2}n(n+1)(2n + 1) \\
S_{n} = \frac{n(n+1)(2n + 1)}{6}
\]
[/latex]

Identity for sum of cubes of first n natural number  : 
[latex]
\[
r^{4} - (r -1)^{4} \\
= r^{4} -  (C(4,0)r^{4}1^{0} - C(4,1)r^{3}1^{1} + C(4,2)r^{2}1^{2} - C(4,3)r^{1}1^{3} + C(4,4)r^{0}1^{4}) \\
= r^{4} - r^{4} + 4r^{3} -6r^{2} + 4r - 1 \\
= 4r^{3} -6r^{2} + 4r - 1
\]
[/latex]



General term from identity sum of cubes of first n natural number :
[latex]
\[
1^{4} - 0^{4} = 4.1^{3} -6.1^{2} + 4.1 - 1 \\
2^{4} - 1^{4} = 4.2^{3} -6.2^{2} + 4.2 - 1 \\
3^{4} - 2^{4} = 4.3^{3} -6.3^{2} + 4.3 - 1 \\
4^{4} - 3^{4} = 4.4^{3} -6.4^{2} + 4.4 - 1 \\
.. .. .. .. .. .. .. .. .. .. .. \\
n^{4} - (n-1)^{4} = 4n^{3} -6 n^{2} + 4n - 1
\]
[/latex]


Sum of cubes of first n natural number : 
[latex]
\[
\text{Adding}, \\
n^{4} = 4(1^{3} + 2^{3} + 3^{3} + .. .. .. + n^{3}) -6(1^{2} + 2^{2} + .. .. + n^{2}) + 4(1 + 2 + 3 + .. ..  + n) -n  \\
n^{4} = 4S_{n} - \frac{6n(n+1)(2n+1)}{6} + \frac{4n(n+1)}{2} - n \\
4S_{n} = n^{4} + n + n(n+1)(2n +1) -2n(n+1) \\
= n(n^{3} + 1) + n(n+1)(2n+1) - 2n(n+1) \\
= n(n+1)(n^{2} - n + 1) + n(n+1)(2n + 1) - 2n(n+1) \\
= n(n+1)(n^{2}-n +1+2n + 1 - 2)\\
= n(n+1)(n^{2} + n) \\
= n^{2}(n+1)^{2} \\
S_{n} = \frac{n^{2}(n+1)^{2}}{4} \\
S_{n} = [\frac{n(n+1)}{2}]^{2}
\]
[/latex]
