Proof of integrating factor reducing to perfect derivative of linear equation  : 
[latex]
\begin{align*}
\frac{dy}{dx} + P.y = Q \\
\text{Multiply both sides by } e^{\int Pdx} \\
e^{\int P dx} \frac{dy}{dx} + e^{\int P dx} Py = Q e^{\int P dx} \\
\frac{d}{dx} y . e^{\int P dx} =  Q . e^{\int p dx}
\end{align*}
[/latex]

Derivation of integrating factor of linear differential equations : 
[latex]
\begin{align*}
\frac{dy}{dx} + Py = Q \\
k \frac{dy}{dx} + kPy = Qk \\
\frac{d}{dx}(y.k) = k \frac{dy}{dx} + k P y \\
y \frac{dk}{dx} + k \frac{dy}{dx} = k \frac{dy}{dx} + k Py \\
\frac{dk}{dx} = kP \\
\frac{dk}{k} = P dx \\
\int \frac{dk}{k} = \int P dx \\
\log_{e}(k) = \int P dx \\
k = e^{\int P dx}
\end{align*}
[/latex]


