Relation between phase difference and path difference  : 
[latex]
\begin{align*}
\text{Path difference } \lambda \text{has phase difference } 2 \pi \\
\text{Path difference } 1 \text{ has phase difference  } \frac{2 \pi}{\lambda} \\
\text{Path difference } x \text{has phase difference } \frac{2 \pi}{\lambda}
\end{align*}
[/latex]

Optical path : 
[latex]
\begin{align*}
c = \frac{d}{t} \\
t = \frac{d}{c} \\
v = \frac{x}{t} \\
t = \frac{x}{v} \\
\frac{x}{v} = \frac{d}{c} \\
d = \frac{x}{v}c \\
d = \frac{c}{v}x \\
d = \mu x
\end{align*}
[/latex]


Equation of resultant superposed wave  : 
[latex]
\begin{align*}
y_{1} = a_{1} \sin \omega t \\
y_{2} = a_{2} \sin \omega t + \phi \\
y = y_{1} + y_{2} \\
y = a_{1} \sin \omega t + a_{2} \sin \omega t + \phi \\
y = a_{1} \sin \omega t + a_{2}( \sin \omega t \cos \phi + \cos \omega t \sin \phi ) \\
y = a_{1} \sin \omega t + a_{2} \sin \omega t \cos \phi + a_{2} \cos \omega t \sin \phi \\
y = (a_{1} + a_{2} \cos \phi) \sin \omega t + a_{2} \cos \omega t \sin \phi \\
A \cos \theta = a_{1} + a_{2} \cos \phi \\
A \sin \theta = a_{2} \sin \phi \\
y = A \sin( \omega t + \theta )
\end{align*}
[/latex]

Equation of resultant amplitude of superposed wave  : 
[latex]
\begin{align*}
A \cos \theta = a_{1} + a_{2} \cos \phi \\
A \sin \theta = a_{2} \sin \phi \\
\text{Squaring and adding} \\
A^{2} = a_{1}^{2} + 2 a_{1}a_{2} \cos \phi + a_{2}^{2} \cos^{2} \phi + a^{2}^{2} \sin^{2} \phi \\
A^{2} = a_{1}^{2} + a_{2}^{2} + 2 a_{1} a_{2} \cos \phi \\
A = \sqrt{ a_{1}^{2} + a_{2}^{2} + 2 a_{1} a_{2} \cos \phi }
\end{align*}
[/latex]

Maximum amplitude of superposed wave  : 
[latex]
\begin{align*}
A_{max} = \sqrt{ a_{1}^{2} + a_{2}^{2} + 2 a_{1} a_{2} } \\
A_{max} = a_{1} + a_{2}
\end{align*}
[/latex]

Minimum amplitude of superposed wave  : 
[latex]
\begin{align*}
A_{min} = \sqrt{ a_{1}^{2} + a_{2}^{2} - 2 a_{1}a_{2}  } \\
A_{min} = | a_{1} - a_{2} |
\end{align*}
[/latex]

Equation of intensity of superposed wave  : 
[latex]
\begin{align*}
A^{2} = a_{1}^{2} + a_{2}^{2} + 2 a_{1} a_{2} \cos \phi \\
I = I_{1} + I_{2} + 2 \sqrt{I_{1} I_{2}} \cos \phi
\end{align*}
[/latex]

Maximum intensity of resultant superposed wave : 
[latex]
\begin{align*}
I_{max} = I_{1} + I_{2} + 2 \sqrt{I_{1} I_{2}} \\
I_{max} = ( \sqrt{I_{1}} + \sqrt{I_{2}} )^{2}
\end{align*}
[/latex]

Minimum intensity of resultant superposed wave  : 
[latex]
\begin{align*}
I_{min} = I_{1} + I_{2} - 2 \sqrt{I_{1}I_{2}} \\
I_{min} = ( \sqrt{I_{1}} - \sqrt{I_{2}} )^{2}
\end{align*}
[/latex]


Phase difference of resultant superposed wave at constructive interference :
[latex]
\begin{align*}
\cos \phi = \text{max} = +1 \\
= \cos n 2 \pi \\
\text{n = 0,1,2, .. .. .. } \\
\phi = n 2 \pi
\end{align*}
[/latex]

Path difference of resultant superposed wave at constructive interference : 
[latex]
\begin{align*}
\text{Path difference} = \frac{\lambda}{2 \pi} 2 \pi n \\
= n \lambda
\end{align*}
[/latex]


Phase difference of resultant superposed wave at destructive interference  : 
[latex]
\begin{align*}
\cos \phi = \text{min} = -1 \\
= \cos \pi(2n + 1) \\
\text{n = 0,1,2, .. .. .. ..} \\
\phi = 2 n \pi + \pi 
\end{align*}
[/latex]

Path difference of resultant superposed wave at destructive interference  : 
[latex]
\begin{align*}
\text{Path difference} = \frac{\lambda}{2 \pi} \pi (2n + 1) \\
= \frac{1}{2} \lambda (2n + 1)
\end{align*}
[/latex]


Path difference between interference fringes : 
[latex]
\begin{align*}
S_2P^{2} - S_1 P^2 = [S_2B^2 + PB^2] - [S_1A^{2} + PA^2] \\
(S_2P - S_1P)(S_2P + S_1P) = [D^2 + (x + \frac{d}{2})^2] - [D^2 + (x - \frac{d}{2})^2] \\
p = \frac{2xb}{2D} \\
p = \frac{xb}{D}
\end{align*}
[/latex]

Position of bright fringes : 
[latex]
\begin{align*}
p = \frac{xb}{D} = n \lambda \\
\frac{xb}{D} = n \lambda \\
x = \frac{n \lambda D}{b} \\
\end{align*}
[/latex]

Position of nth dark fringe : 
[latex]
\begin{align*}
p = \frac{xb}{D} = (2n - 1)\frac{\lambda}{2} \\
\frac{xb}{D} = (2n - 1) \frac{\lambda}{2} \\
x = (2n - 1) \frac{ \lambda D }{2b}
\end{align*}
[/latex]

Fringe width : 
[latex]
\begin{align*}
\beta = \frac{(n+1)\lambda D}{b} - \frac{n \lambda D}{b} \\
= n \frac{\lambda D}{b} - \frac{n \lambda D }{b}  \\
= \frac{\lambda D}{b} \\
\end{align*}
[/latex]

Angular width of fringe : 
[latex]
\begin{align*}
\theta = \frac{\beta}{D} \\
\theta = \frac{\lambda D}{b D} \\
\theta = \frac{\lambda}{b}
\end{align*}
[/latex]

Fringe width in relation with refractive index : 
[latex]
\begin{align*}
\lambda^{|} = \frac{\lambda}{\mu} \\
\beta^{|} = \frac{\lambda^{|} D}{b} \\
\beta^{|} = \frac{\lambda D}{ \mu b } \\
\beta^{|} = \frac{\beta}{\mu}
\end{align*}
[/latex]












