<<<
 Expression for expansion of euler's number raised to the power of x in algebra
---


$$ e^{x} = 1 + \frac{x}{1!} + \frac{x^{2}}{2!} + \frac{x^{3}}{3!} + .. .. .. + \frac{x^{r}}{r!} + .. .. .. \infty $$ 


>>> 
<<<
 Proof for the expansion of euler's number raised to the power x in algebra
---


- $$ \text{If } n > 1 \text{ then } \frac{1}{n} < 1 $$
- $$ (1 + \frac{1}{n})^{nx} = 1 + nx . \frac{1}{n} + \frac{nx.(nx-1)}{2!}. \frac{1}{n^{2}} + \frac{nx. (nx-1) (nx-2)}{3!} \frac{1}{n^{3}} + .. .. $$
- $$ (1 + \frac{1}{n})^{nx} = 1 + x + \frac{x(x - \frac{1}{n})}{2!} + \frac{x(x - \frac{1}{n})(x - \frac{2}{n})}{3!} + .. .. $$ 
- On infinitely large value of n
- $$ (1 + \frac{1}{n})^{nx} = 1 + x + \frac{x^{2}}{2!} + \frac{x^{3}}{3!}+ .. .. .. $$ 
- $$ x = 1 $$ 
- $$ \lim_{n \rightarrow \infty} ( 1 + \frac{1}{n} )^{n} = 1 + \frac{1}{1!} + \frac{1}{2!} + \frac{1}{3!} + â€¦ = e $$
- $$ ( 1 + \frac{1}{n} )^{nx} = {(1 + \frac{1}{n})}^{x} = e^{x} \text{as} e^{x} \rightarrow \infty $$ 
- $$ e^{x} = 1 + \frac{x}{1!} + \frac{x^{2}}{2!} + \frac{x^{3}}{3!} + .. .. .. + \frac{x^{r}}{r!} + .. .. .. \infty $$ 


>>> 
<<<
 Expression for the expansion of euler's number raised to the power -x in algebra
---


$$ e^{-x} = 1 - \frac{x}{1!} + \frac{x^{2}}{2!} - \frac{x^{3}}{3!} + .. .. .. .. .. + (-1)^{r} \frac{x^{r}}{r!} + .. .. ..  $$ 

>>> 
<<<
 Expression for expansion of euler's number in algebra
---


$$ e = 1 + \frac{1}{1!} + \frac{1}{2!} + \frac{1}{3!} + .. .. ..  $$ 


>>> 
<<<
 Expression for expansion of euler's number raised to the power -1 in algebra
---

$$ e^{-1} = 1 - \frac{1}{1!} + \frac{1}{2!} - \frac{1}{3!} + .. .. ..  $$ 

>>> 
<<<
 Scope of exponential series in algebra
---

All values of x




>>> 
