<<<
 Expression for expansion of a constant raised to the power of x
---

$$ a^{x} = 1 + \frac{x}{1!} \log_{e}a + \frac{x^{2}}{2!}(\log_{e}a)^{2} + ..  .. .. .. + \frac{x^{r}}{r!}( \log_{e}(a) )^{r} + .. .. .. \text{to} \infty $$ 

>>> 
<<<
 Scope of application of expansion of constant raised to the power of x
---

All values of x



>>> 
<<<
 Proof for the expansion of a constant raised to the power of x
---

- $$ a = e^{k} $$
- $$ k = \log_{e}(a) $$
- $$ a^{x} = (e^{k})^{x} = e^{kx} $$
- $$ a^{x} = 1 + \frac{kx}{1!} + \frac{(kx)^{2}}{2!} + .. .. .. + \frac{(kx)^{r}}{r!} + .. .. .. \text{to} \infty $$ 
- $$ a^{x} = 1 + \frac{x}{1!} \log_{e}a + \frac{x^{2}}{2!}(\log_{e}a)^{2} + ..  .. .. .. + \frac{x^{r}}{r!} ( \log_{e}a)^{r} + .. .. .. \text{to} \infty $$ 



>>> 
